Extract definition typing from member typing, plus automation
We'll soon want to add semantic definition typing and relate it to semantic
value typing. So, split out what I'm gonna need for definitions.

Proofs of affected semantic lemmas needed to be almost rewritten.

Some trivial Coq proof steps can be automated, and automation reduces the work
to deal with such trivial changes, so import (some of) my homegrown tactics for
that.

theories/operational.v
@@ -2,6 +2,7 @@ From iris.program_logic Require Export ectx_language ectxi_language.
 From iris.algebra Require Export ofe.
 
 Require Export Dot.dotsyn.
+Require Import Dot.tactics.
 
 Module lang.
 
@@ -46,14 +47,38 @@ Notation "s .[ v /]" := (s .[ v .: var_vl ])
     variable). To use when descending under the [vobj] binder. *)
 Definition selfSubst (ds: dms): dms := ds.[vobj ds/].
 
+Definition obj_opens_to v ds: Prop :=
+  ∃ ds', v = vobj ds' ∧ selfSubst ds' = ds.
+Notation "v ↗ ds" := (obj_opens_to v ds) (at level 20).
+
+(* Instead of letting obj_opens_to autounfold, provide tactics to show it's deterministic and *)
+
+(** Rewrite v ↗ ds to vobj ds' ↗ ds. *)
+Ltac simplOpen ds' :=
+  lazymatch goal with
+  | H: ?v ↗ ?ds |-_=>
+    inversion H as (ds' & -> & _)
+  end.
+
+(** Determinacy of obj_opens_to. *)
+Lemma openDet v ds1 ds2: v ↗ ds1 -> v ↗ ds2 -> ds1 = ds2.
+Proof.
+  rewrite /obj_opens_to; intros; ev; by optFuncs_det.
+Qed.
+Ltac openDet :=
+  lazymatch goal with
+  | H1: ?v ↗ ?ds1, H2: ?v ↗ ?ds2 |- _=>
+    assert (ds1 = ds2) as <- by (eapply openDet; eassumption)
+  end.
+
 Definition dms_proj_val ds l v: Prop :=
-  index_dms l (selfSubst ds) = Some (dvl v).
+  index_dms l ds = Some (dvl v).
 
 Inductive head_step : tm -> state -> list observation -> tm -> state -> list tm -> Prop :=
 | st_beta : forall t1 v2,
     head_step (tapp (tv (vabs t1)) (tv v2)) tt [] (t1.[v2/]) tt []
 | st_proj : forall ds l v,
-    dms_proj_val ds l v ->
+    dms_proj_val (selfSubst ds) l v ->
     head_step (tproj (tv (vobj ds)) l) tt [] (tv v) tt []
 .
 
