theories/tactics.v
@@ -1,0 +1,107 @@
+(* Remove Hints Bool.trans_eq_bool. *)
+
+Ltac inverse H := (inversion H; subst).
+Ltac int := intuition trivial.
+
+Ltac ev := repeat match goal with
+                    | H: exists _, _ |- _ => destruct H
+                    | H: _ /\  _ |- _ => destruct H
+                    | H : exists2 _, _ & _ |- _ => destruct H
+                    | H : { _ | _ } |- _ => destruct H
+                    | H : { _ | _ & _ } |- _ => destruct H
+                    (* | H : { _ & _ } |- _ => destruct H *)
+                    | H : { _ : _ & _ & _ } |- _ => destruct H
+                    | p : _ * _ |- _ => destruct p
+                  end.
+
+(* Avoid case distinctions when we know the right case from the hypotheses.
+   Otherwise, we end up with branches where the context says that ?x = A and ?x
+   = B, with A and B incompatible, and must use discriminate to remove those
+   branches. *)
+Ltac better_case_match :=
+  match goal with
+  | H : context [ match ?x with _ => _ end ] , H1 : _ = ?x |- _ =>
+    rewrite <- H1 in H
+  | H : context [ match ?x with _ => _ end ] , H1 : ?x _ |- _ =>
+    rewrite H1 in H
+  | H : context [ match ?x with _ => _ end ] |- _ =>
+    destruct x eqn:?
+
+  | H1 : _ = ?x |- context [ match ?x with _ => _ end ] =>
+    rewrite <- H1
+  | H1 : ?x = _ |- context [ match ?x with _ => _ end ] =>
+    rewrite H1
+  | |- context [ match ?x with _ => _ end ] =>
+    destruct x eqn:?
+  end.
+
+(* From Chlipala's tactics. *)
+Ltac cinject H := injection H; clear H; intros; subst.
+
+(* Apply automatically injection on hypotheses of form ?c args1 = ?c args2; if c
+   is a constructor this will produce equalities args1_i = args2_i for all i.
+   Since this tactic uses injection, it is more reliable than attempts based on
+   inversion. *)
+Ltac injectHyp :=
+  match goal with
+  | H : ?c _ _ _ _ _ _ = ?c _ _ _ _ _ _ |- _ => cinject H
+  | H : ?c _ _ _ _ _ = ?c _ _ _ _ _ |- _ => cinject H
+  | H : ?c _ _ _ _ = ?c _ _ _ _ |- _ => cinject H
+  | H : ?c _ _ _ = ?c _ _ _ |- _ => cinject H
+  | H : ?c _ _ = ?c _ _ |- _ => cinject H
+  | H : ?c _ = ?c _ |- _ => cinject H
+  | H : ?c = ?c |- _ => clear H
+  end.
+Ltac injectHyps := repeat injectHyp.
+
+Ltac optFuncs_det :=
+  match goal with
+  | H1 : ?t = _, H2 : ?t = _ |- _ =>
+    let H := fresh "H" in
+    rewrite H2 in H1; injectHyps
+  end.
+
+(* To use with repeat fequalSafe in automation.
+   Unlike f_equal, won't try to prove a = b = c + d by a = c and b = d --- such
+   equaities are omega's job. *)
+Ltac fequalSafe :=
+  match goal with
+  | [ |- Some _ = Some _ ] => f_equal
+  | [ |- (_, _) = (_, _) ] => f_equal
+  end.
+
+Hint Constructors option.
+Hint Constructors list.
+
+Hint Resolve ex_intro.
+
+(** Support writing external hints for lemmas that must not be applied twice for a goal. *)
+(* The usedLemma and un_usedLemma marker is taken from Crush.v (where they were called done and un_done). *)
+
+(** Devious marker predicate to use for encoding state within proof goals *)
+Definition usedLemma {T : Type} (x : T) := True.
+
+(** After a round of application with the above, we will have a lot of junk [usedLemma] markers to clean up; hence this tactic. *)
+Ltac un_usedLemma :=
+  repeat match goal with
+           | [ H : usedLemma _ |- _ ] => clear H
+         end.
+Ltac markUsed H := assert (usedLemma H) by constructor.
+
+Ltac try_once lm :=
+    match goal with
+    | H : usedLemma lm |- _ => fail 1
+    | _ => markUsed lm; eapply lm
+    end.
+
+Ltac better_case_match_ex := try better_case_match; injectHyps; try discriminate.
+
+Tactic Notation "try_once_tac" constr(T) tactic(tac) :=
+  match goal with
+  | H : usedLemma T |- _ => fail 1
+  | _ => markUsed T; tac
+  end.
+
+(* Example. *)
+(* Definition injectHyps_marker := 0. *)
+(* Hint Extern 5 => try_once_tac injectHyps_marker injectHyps. *)
